src/verified_adapter.mli
@@ -5,6 +5,7 @@ open Helper
 
 val is_monitorable: Db.schema -> formula -> bool * (formula * string) option
 val convert_formula: Db.schema -> formula -> Verified.Monitor.formula
-val convert_db: monpolyData -> (Verified.Monitor.char list ->
-  Verified.Monitor.event_data list Verified.Monitor.set list option) * Verified.Monitor.nat
+val convert_db: monpolyData -> (Verified.Monitor.char list,
+  Verified.Monitor.event_data list Verified.Monitor.set list) Verified.Monitor.mapping *
+  Verified.Monitor.nat
 val convert_violations: (Verified.Monitor.nat * Verified.Monitor.event_data option list Verified.Monitor.set) list -> (int * relation) list
