thys/Monitor_Code.thy
@@ -70,17 +70,23 @@ lemma image_these: "f ` Option.these X = Option.these (map_option f ` X)"
 thm default_maux.meval.simps(2)
 
 lemma meval_MPred: "meval n t db (MPred e ts) =
-  (case db e of None \<Rightarrow> [{}] | Some Xs \<Rightarrow> map (\<lambda>X. \<Union>v \<in> X.
+  (case Mapping.lookup db e of None \<Rightarrow> [{}] | Some Xs \<Rightarrow> map (\<lambda>X. \<Union>v \<in> X.
   (set_option (map_option (\<lambda>f. Table.tabulate f 0 n) (match ts v)))) Xs, MPred e ts)"
   by (force split: option.splits simp: Option.these_def image_iff)
 
 lemmas meval_code[code] = default_maux.meval.simps(1) meval_MPred default_maux.meval.simps(3-)
 
-definition mk_db :: "(string \<times> event_data list) list \<Rightarrow> _" where
-  "mk_db = Monitor.mk_db o set"
+definition mk_db :: "('t \<Rightarrow> Formula.name list) \<Rightarrow> ('t \<Rightarrow> Formula.name \<Rightarrow> event_data list set) \<Rightarrow> 't \<Rightarrow> _" where
+  "mk_db get_names get_table t = Monitor.mk_db (\<Union>n \<in> set (get_names t). (\<lambda>v. (n, v)) ` get_table t n)"
 
 definition rbt_fold :: "_ \<Rightarrow> event_data tuple set_rbt \<Rightarrow> _ \<Rightarrow> _" where
   "rbt_fold = RBT_Set2.fold"
+
+definition rbt_empty :: "event_data list set_rbt" where
+  "rbt_empty = RBT_Set2.empty"
+
+definition rbt_insert :: "_ \<Rightarrow> _ \<Rightarrow> event_data list set_rbt" where
+  "rbt_insert = RBT_Set2.insert"
 
 lemma saturate_commute:
   assumes "\<And>s. r \<in> g s" "\<And>s. g (insert r s) = g s" "\<And>s. r \<in> s \<Longrightarrow> h s = g s"
@@ -406,12 +412,14 @@ lemma remove_Union_code[code]: "remove_Union A X B =
   apply (transfer fixing: A X B)
   using remove_Union_finite[of X A B] by (auto simp add: remove_Union_def)
 
-lemma mk_db_code[code]: "mk_db xs p =
-    (case List.map_filter (\<lambda>(p',ts). if p = p' then Some ts else None) xs of
-    [] \<Rightarrow> None | xs \<Rightarrow> Some [set xs])"
-  unfolding mk_db_def Monitor.mk_db_def
-  by (auto 0 3 simp: map_filter_def filter_empty_conv filter_eq_Cons_iff image_iff
-    split: list.splits option.splits if_splits prod.splits)
+lemma mk_db_code[code]:
+  "mk_db get_names get_table t =
+    Mapping.of_alist (List.map_filter
+      (\<lambda>n. let X = get_table t n in if X = {} then None else Some (n, [X])) (get_names t))"
+  unfolding mk_db_def map_filter_def Let_def
+  by (transfer fixing: get_names get_table t, subst list.map_cong[OF refl, of _ _ "\<lambda>n. (n, [get_table t n])"])
+    (auto simp: fun_eq_iff map_of_map_restrict image_iff restrict_map_def)
+ 
 
 declare [[code drop: New_max_getIJ_genericJoin New_max_getIJ_wrapperGenericJoin]]
 declare New_max.genericJoin.simps[folded remove_Union_def, code]
@@ -423,9 +431,10 @@ export_code convert_multiway minit_safe mstep mmonitorable_exec
 export_code
   (*basic types*)
   nat_of_integer integer_of_nat int_of_integer integer_of_int enat
-  String.explode String.implode interval mk_db RBT_set rbt_fold EInt
+  String.explode String.implode interval mk_db
+  RBT_set rbt_empty rbt_insert rbt_fold
   (*term, formula, and regex constructors*)
-  Formula.Var Formula.Agg_Cnt Formula.Pred Regex.Skip Regex.Wild
+  EInt Formula.Var Formula.Agg_Cnt Formula.Pred Regex.Skip Regex.Wild
   (*main functions*)
   convert_multiway minit_safe mstep mmonitorable_exec
   in OCaml module_name Monitor file_prefix "verified"
